$$10^{10}
2^{n+1}
{(n+1)}^2
\sqrt{1-x^2}
\overline{x+\overline{z}}
p{}^{e_1}_1
a_{b_{c_{d_e}}}
\root 3 \of {h''_n(\alpha{}x}
$$


Deleting an element from an $n$-tuple leaves an $(n-1)$-tuple.

%Letters that extend below the baseline:
%gjpqQfy

$
z^{*{}2}
h'_*(z)
$

$x := 4+y$

$12{,}345,567$

$13{.}3.56$

$e^{-x^2}$

$D \sim p^{\alpha}M + l$

$\hat{g}{\in}(H^{{\pi}^{-1}}_1)'$

$1\over{2}$

$n+1\over{3}$

$n+1\choose{3}$

$$\sum_{n=1}^3{} Z_n^2$$

$x + y^{2\over{k+1}}$

$x + y^{2/(k+1)}$

${a+1\over{b+1}}x$

$((a+1)/(b+1))x$

$$x = {y^2\over k+1}$$

$7{1\over2}asdf$

$$\sqrt{p^{e'}_2}$$

$$n +\scriptstyle{n} + \scriptscriptstyle{n}$$

You can do this, but its bad.

$${n\choose{k}}\over{2}$$

Alternatives are:

$${1\over{2}}{n\choose{k}}$$
or
$${\displaystyle{n\choose{k}}}\over{2}$$

$${p\choose{2}} x^2 y^{p-2} - {1\over{1-x}} {1\over{1-x^2}}$$


For stuff like summations, thers a big difference between \$ and \$\$.

With just \$ (in text style), you get $\sum{x_n}$, but with display style, you get $$\sum{x_n}$$
%

 $$\sum^p_{i=1}{\sum^q_{j=1}{\sum^r_{k=1}}
 {a_{ij}b_{jk}c_{ki}}}$$

$$\sum_{{1\ge{}i\ge{}p}\atop{{1\ge{}j\ge{}q}\atop{{1\ge{}k\ge{}r}}}}{a_{ij}b_{jk}c_{ki}}$$


$$
\biggl{(} {\partial{}^2\over{\partial{}x^2}} + {\partial{}^2\over{\partial{}y^2}}\biggl{)}
{\bigl|\varphi(x + iy)\bigl|}^2
$$

$\bigl( x + f(x)\bigr) \big/ \bigl( x - f(x) \bigr)$
%
%{{\phi(k)}\over{k-1}}}}

$$\pi(n) = 
    {\sum^n_{k=2}
    {\left\lfloor{{\phi(k)}\over{k-1}}\right\rfloor}}
$$


$$
\pi(n) =
{\sum^n_{m=2}{
    \left\lfloor
    \bigg(
    \sum^{m-1}_{k=1}
	\left\lfloor
	(m/k) \big/ \lceil m/k \rceil
	\right\rfloor
    \bigg)
    ^{-1}
    \right\rfloor}
}
$$

$R(n,t) = O(t^{n/2})$, as $t \rightarrow 0^+$
$R(n,t) = O(t^{n/2})$, as $t \to 0^+$

$\sin(2\theta)$

$$\lim_{x \to 0}{\sin(x)\over{x}} = 1$$

$$p_1(n) = 
    \lim_{m \to \infty} 
	\sum^\infty_{\nu=0}
	{
	    \bigl( 1-\cos^{2m} 
		(\nu!^n\pi\big/n)
	    \bigr)
	}
$$

$\sqrt{\hbox{Stuff in roman font}(x)}$
$\sqrt{\rm{Stuff\ in\ roman\ font}(x)}$

$${n\choose k} \equiv 
    {{\lfloor n/p \rfloor} \choose{\lfloor k/p \rfloor}}
    {{n \bmod p} \choose {k \bmod p}}
    \pmod p
$$


$\bf\bar x^{\rm T}Mx={\rm 0}\iff x=0$

$S \subseteq{\mit\Sigma} \iff S \in{\cal S}$

$${\it available} + \sum^n_{i=1} \max
    \bigl( {\it full}(i), {\it reserved}(i) \bigr)
= {\it capacity}$$

Let $H$~be a Hilbert~space, $C$~a closed bounded convex subset of~$H$, \ 
$T$~a nonexpansive self~map of~$C$. Suppose that as $n \to \infty$,\ $a_{n,k} \to 0$
for each~$k$, and 
    $\gamma_n = \sum^\infty_{k=0} (a_{n,k+1} - a_{n_k} )^+ \to 0$.
Then for each $x$~in~$C$, 
    $A_nx=\sum^\infty_{k=0}a_{n,k}T^kx$
converges weakly to a fixed point of~$T$.



$$\int^\infty_0 {{t-ib}\over{t^2+b^2}} e^{iat} \, dt =
    e^{ab}E_1(ab),
    \qquad
    a,b>0.
$$


$18\, {\rm mi/hr}$

$\bar{h} = 1.0545 \times 10^{-27} \rm \, erg \, sec$.

$x_1 + x_1x_2 + \cdots + x_1x_2\ldots x_n$

$(x_1,\ldots, x_n) \cdot (y_1,\ldots, y_n) = x_1y_1 + \cdots + x_ny_n$

Well $\ldots\,$, hardly ever

$\{\, x \mid x > 5 \, \}$

$\bigl\{ \,x^3 \mid h(x) \in \{\, -1, 0, +1 \} \bigr\}$

$$
f(x) = \cases{   1/3   &if $0 \le x \le 1$;\cr
	        2/3   &if $3 \le x \le 4$;\cr
		0     &elsewhere.\cr
	    }
$$



$$\overbrace{x + y}^{k\rm\; times}$$

$$
\left\lgroup
    \matrix{
	a&b&c	\cr
	d&e&f	\cr
	}
\right\rgroup
\left\lgroup
    \matrix{
	u&x	\cr
	v&y	\cr
	w&z	\cr
    }
\right\rgroup
$$

$$A = 
\pmatrix{
    a_{11} & a_{12} & \ldots & a_{1n}	    \cr
    a_{21} & a_{22} & \ldots & a_{2n}	    \cr
    \vdots & \vdots & \ddots & \vdots	    \cr
    a_{m1} & a_{m2} & \ldots & a_{mn}	    \cr
    }
$$

$$
\pmatrix{
    y_1	    \cr
    \vdots  \cr
    y_k	    \cr
}
$$
$$X_n = X_k \qquad \hbox{if and only if} \qquad Y_n = Y_k \quad \hbox{and} \quad Z_n = Z_k$$

$$Y_n = X_n \bmod p \qquad \hbox{and}$$

$$\sum^\infty_{n=0} a_nz^n \qquad \hbox{converges if} \qquad |z|< 
    \Bigl( {\limsup_{n\to\infty}} \root n\! \of{|a_n|}\, \Bigr)^{-1}
$$

$$
{{f(x+\Delta x) -f(x)}\over{\Delta x}} \to f'(x) \qquad \hbox{as $\Delta x \to 0$}
$$

$$
\Vert u_i \Vert = 1, \qquad u_i \cdot u_j = 0 \quad \hbox{if $i \not= j$}
$$

$$
\hbox{\it The confluent image of}\quad
\left\{
    \matrix{
    \hbox{\it an arc} \cr
    \hbox{\it a circle} \cr
    \hbox{\it an arc} \cr
    }
\right\}
\quad\hbox{\it is}\quad
\left\{
    \matrix{
    \hbox{\it an arc}\hfill \cr
    \hbox{\it an arc or a circle}\hfill \cr
    \hbox{\it a fan or an arc}\hfill \cr
    }
\right\}
$$

$$\hbox{$y={1\over2} x$}$$
$$\textstyle y={1\over2} x$$

$$\leftline{\indent$\displaystyle 1-{1\over2} + {1\over3} - {1\over4} + \cdots = \ln2$}$$

$$x+y = y + x \eqno(9)$$
$$x+y = y + x \leqno n^2$$

$$
\prod_{k\ge0}
    {1\over(1-q^kz)} =
    \sum_{n\ge0}
	z^n
    \bigg/\!\!
    \prod_{1\le k\le  n}
	(1-q^k)
    .
    \eqno(16')
$$

$$
x + n = n + x \eqno\hbox{(3--1)}
$$

$$
\eqalign{
    X_1 + \cdots + X_p &=m, \cr
    Y_1 + \cdots + Y_q &=n, \cr
}
$$

$$
\eqalign{
    T(n) \le T(2^{\lceil\lg n\rceil}) 
    &\le c(3^{\lceil\lg n \rceil} - 2^{\lceil\lg n \rceil})\cr
    &< 3c \cdot 3^{\lg n}\cr
    &= 3c\,n^{\lg 3}.\cr
    }
$$

$$
\eqalign{
P(x) &= a_0 + a_1x + a_2^2 + \cdots + a_nx^n\cr
P(-x) &= a_0 - a_1x + a_2^2 - \cdots + (-1)^na_nx^n\cr
}
\eqno(30)
$$

$$
\leqalignno{
    \gcd(u, v) &= \gcd(v, u);&(9)\cr
    \gcd(u, v) &= \gcd(-u, v). &(10)\cr
}
$$

$$
\eqalignno{
    \left( \int^\infty_\infty e^{-x^2} \,dx \right)^2
    & = \int^\infty_{-\infty} \int^\infty_{-\infty} e^{-(x^2+y^2)} \, dx \, dy \cr
    & = \int^{2\pi}_0 \!\! \int^\infty_0 e^{-r^2} r \, dr \, d\theta \cr
    & = \int^{2\pi}_0
	\left(
	    -{e^{-r^2}\over2} \bigg|^{r=\infty}_{r=0}
	\right)
	\, d\theta \cr
    & = \pi. & (11)\cr
}
$$

$$\displaylines{
    \hfill x\equiv x; \hfill\llap(1) \cr
    \hfill \hbox{if}\quad x\equiv y \quad \hbox{then} \quad y \equiv x;\hfill\llap(2)\cr
    \hfill \hbox{if}\quad x\equiv y \quad \hbox{and} \quad y\equiv z \quad \hbox{then} \quad y \equiv z.\hfill\llap(3) \cr
}
$$

$$
\eqalignno{
    x_nu_1+ \cdots+ x_{n+t-1}u_t 
	&= x_nu_1 + (ax_n + c)u_2 + \cdots \cr
	&\qquad + \bigl(a^{t-1}x_n + c(a^{t-2} + \cdots + 1)\bigr)u_t \cr
	&= (u_1 + au_2 + \cdots + a^{t-1}u_t) x_n + h(u_1, \ldots, u_t).&(47)
    }
$$

$$
\displaylines{
    \quad\sum_{1\le j\le n}
	{1\over
	    (x_j-x_1) \ldots (xj-x_{j-1})(x-x_j)(x_j-x_{j+1}) \ldots (x_j-x_n)
	}
    \hfill \cr
    \hfill 
	= {1\over
	    (1-x_1)\ldots(x-x_n)}.\quad\llap(27).
}
$$





\end
